Basis for the CLEAN embedding

C11-FrontEnd/semantic-backends/CLEAN/Clean.thy
@@ -1,1 +1,583 @@
-../../../../src/Clean.thy
+(*****************************************************************************
+ * MonadicPrograms.thy --- a base testing theory for programs.
+ * Burkhart Wolff and Chantal Keller, LRI, Univ. Paris-Sud, France
+ ******************************************************************************)
+
+
+chapter {* The Clean Language *}
+
+theory Clean
+  imports Symbex_MonadSE
+          "~~/src/HOL/Eisbach/Eisbach"
+  keywords "global_vars" "local_vars" :: thy_decl 
+(*
+     and "funct" :: thy_decl
+
+     and "pre" "post" (* "local_vars" *)
+     and "returns" 
+     and "end_funct" :: thy_goal
+*)
+begin
+  
+  
+text{* Clean is a minimalistic imperative language 
+with C-like control-flow operators based on a shallow embedding into the
+SE exception Monad theory formalized in @{theory MonadSE}. It comprises:
+\begin{itemize}
+\item C-like control flow with \verb+break+ and \verb+return+
+\item global variables
+\item function calls (seen as Monad-executions) with side-effects, recursion
+      and local variables
+\item parameters are modeled via functional abstractions 
+      (functions are Monads ...); a passing of parameters to local variables
+      might be added later
+\item cartouche syntax for update operations.
+\end{itemize} *}
+  
+  
+chapter {* Proof of concept for a monadic symbolic execution calculus for WHILE programs *}
+
+
+section\<open> Control-States  \<close>
+  
+record 'a control_state = 
+          break_val :: bool
+          return_val :: "'a option"
+          
+typ "('a, 'b) control_state_ext"
+
+ML\<open> 
+fun typ_2_string_raw (Type(s,S)) = 
+        let  val h = if null S then "" else enclose "(" ")" (commas (map typ_2_string_raw S)) ;
+        in h ^ s end
+   |typ_2_string_raw (TFree(s,_))  = s 
+   |typ_2_string_raw (TVar((s,n),_))  = s^(Int.toString n) ;
+
+typ_2_string_raw @{ typ "('a, 'b) control_state_ext"}
+\<close>
+
+record 'a mmm = "'a control_state" +
+       df :: "int"
+
+record 'a mmk = "'a mmm" + dsf :: int 
+
+(* break quites innermost while or for, return quits an entire execution sequence. *)  
+definition break :: "(unit, ('\<alpha>, '\<sigma>) control_state_ext) MON\<^sub>S\<^sub>E"
+  where   "break \<equiv> (\<lambda> \<sigma>. Some((), \<sigma> \<lparr> break_val := True \<rparr>))"
+  
+definition unset_break :: "(unit, ('\<alpha>, '\<sigma>) control_state_ext) MON\<^sub>S\<^sub>E"
+  where   "unset_break \<equiv> (\<lambda> \<sigma>. Some((), \<sigma> \<lparr> break_val := False \<rparr>))"
+
+definition return :: "'\<alpha> \<Rightarrow> (unit, ('\<alpha>, '\<sigma>) control_state_ext) MON\<^sub>S\<^sub>E"    
+  where   "return x = (\<lambda> \<sigma>. Some((), \<sigma> \<lparr> return_val := Some x \<rparr>))"
+    
+definition unset_return_val :: "('\<alpha>, ('\<alpha>, '\<sigma>) control_state_ext) MON\<^sub>S\<^sub>E"    
+  where   "unset_return_val  = (\<lambda> \<sigma>. Some(the (return_val \<sigma>), \<sigma> \<lparr> return_val := None \<rparr>))"
+    
+definition exec_stop :: "('\<alpha>, '\<sigma>) control_state_ext \<Rightarrow> bool"
+  where   "exec_stop = (\<lambda> \<sigma>. break_val \<sigma> \<or> return_val \<sigma> \<noteq> None)"
+
+text\<open> A "lifter" that embeds a state transformer into the state-exception monad. \<close>
+
+consts syntax_assign :: "('\<alpha>  \<Rightarrow> int) \<Rightarrow> int \<Rightarrow> term" (infix ":=" 60)
+
+definition assign :: "(('\<alpha>, '\<sigma>) control_state_scheme  \<Rightarrow> 
+                       ('\<alpha>, '\<sigma>) control_state_scheme) \<Rightarrow> 
+                       (unit,('\<alpha>, '\<sigma>) control_state_scheme)MON\<^sub>S\<^sub>E"
+where     "assign f = (\<lambda>\<sigma>. if exec_stop \<sigma> 
+                              then Some((), \<sigma>)  
+                              else Some((), f \<sigma>))"
+
+    
+definition if_C :: "[('\<alpha>, '\<sigma>) control_state_ext \<Rightarrow> bool, 
+                      ('\<beta>, ('\<alpha>, '\<sigma>) control_state_ext)MON\<^sub>S\<^sub>E, 
+                      ('\<beta>, ('\<alpha>, '\<sigma>) control_state_ext)MON\<^sub>S\<^sub>E] \<Rightarrow> ('\<beta>, ('\<alpha>, '\<sigma>) control_state_ext)MON\<^sub>S\<^sub>E"
+  where   "if_C c E F = (\<lambda>\<sigma>. if exec_stop \<sigma> 
+                              then Some(undefined, \<sigma>)  (* state unchanged, return arbitrary *)
+                              else if c \<sigma> then E \<sigma> else F \<sigma>)"     
+
+syntax    (xsymbols)
+          "_if_SECLEAN" :: "['\<sigma> \<Rightarrow> bool,('o,'\<sigma>)MON\<^sub>S\<^sub>E,('o','\<sigma>)MON\<^sub>S\<^sub>E] \<Rightarrow> ('o','\<sigma>)MON\<^sub>S\<^sub>E" 
+          ("(if\<^sub>C _ then _ else _fi)" [5,8,8]8)
+translations 
+          "(if\<^sub>C cond then T1 else T2 fi)" == "CONST Clean.if_C cond T1 T2"
+
+          
+          
+definition while_C :: "(('\<alpha>, '\<sigma>) control_state_ext \<Rightarrow> bool) 
+                        \<Rightarrow> (unit, ('\<alpha>, '\<sigma>) control_state_ext)MON\<^sub>S\<^sub>E 
+                        \<Rightarrow> (unit, ('\<alpha>, '\<sigma>) control_state_ext)MON\<^sub>S\<^sub>E"
+  where     "while_C c B \<equiv> (\<lambda>\<sigma>. if exec_stop \<sigma> then Some((), \<sigma>)
+                                 else ((MonadSE.while_SE (\<lambda> \<sigma>. \<not>exec_stop \<sigma> \<and> c \<sigma>) B) ;- 
+                                       unset_break) \<sigma>)"
+  
+syntax    (xsymbols)
+          "_while_C" :: "['\<sigma> \<Rightarrow> bool, (unit, '\<sigma>)MON\<^sub>S\<^sub>E] \<Rightarrow> (unit, '\<sigma>)MON\<^sub>S\<^sub>E" 
+          ("(while\<^sub>C _ do _ od)" [8,8]8)
+translations 
+          "while\<^sub>C c do b od" == "CONST Clean.while_C c b"
+
+definition body\<^sub>C :: "   (unit, ('\<alpha>, '\<sigma>) control_state_ext)MON\<^sub>S\<^sub>E
+                     \<Rightarrow> ('\<alpha>, ('\<alpha>, '\<sigma>) control_state_ext)MON\<^sub>S\<^sub>E
+                     \<Rightarrow> (unit, ('\<alpha>, '\<sigma>) control_state_ext)MON\<^sub>S\<^sub>E  
+                     \<Rightarrow> ('\<alpha>,   ('\<alpha>, '\<sigma>) control_state_ext)MON\<^sub>S\<^sub>E"
+  where   "body\<^sub>C push pop X \<equiv> (push ;- X ;- unset_break ;- (x \<leftarrow> pop; unset_return_val;- unit\<^sub>S\<^sub>E(x)))"     
+    
+(* a "function m (x1:T1; ... ;xn : Tn) : T = {locvar-decl; X}" is then
+   compiled to:
+
+   a) an extension of the ('\<alpha>, '\<sigma>) cstate_ext with the locvar-decl-stack 
+      and the corresponding generation of the push and pop operations on that stack
+ 
+   b) definition m\<^sub>S\<^sub>E :: " T1 \<Rightarrow> ... \<Rightarrow> Tn \<Rightarrow> T" 
+        where m\<^sub>S\<^sub>E x1 .. xn \<equiv> body\<^sub>C push\<^sub>l\<^sub>o\<^sub>c\<^sub>v\<^sub>a\<^sub>r\<^sub>-\<^sub>d\<^sub>e\<^sub>c\<^sub>l pop\<^sub>l\<^sub>o\<^sub>c\<^sub>v\<^sub>a\<^sub>r\<^sub>-\<^sub>d\<^sub>e\<^sub>c\<^sub>l X
+
+   CAVEAT: This coding scheme has the undesired effect that all return types of functions must be 
+   the same ;-( But as a first shot, this is perhaps acceptable.
+*)   
+    
+section\<open> A Specialized Representation of States based on Records) \<close>
+
+ML{*
+
+structure StateMgt_core = 
+struct
+
+val control_stateT = @{typ "('a) control_state"};
+
+fun merge_control_stateT (@{typ "('a) control_state"},t) = t
+   |merge_control_stateT (t, @{typ "('a) control_state"}) = t
+   |merge_control_stateT (t, t') = if (t = t') then t else error"can not merge CLEAN state"
+
+datatype var_kind = global_var of typ | local_var of typ
+
+fun type_of(global_var t) = t | type_of(local_var t) = t
+
+type state_field_tab = var_kind Symtab.table
+
+structure Data = Generic_Data
+(
+  type T       = (state_field_tab * typ) 
+  val  empty   = (Symtab.empty,control_stateT)
+  val  extend  = I
+  fun  merge((s1,t1),(s2,t2))  = (Symtab.merge (op =)(s1,s2),merge_control_stateT(t1,t2))
+);
+
+
+val get_data        = Data.get o Context.Proof;
+val map_data        = Data.map;
+val get_data_global = Data.get o Context.Theory;
+val map_data_global = Context.theory_map o map_data;
+
+val get_state_type          = snd o get_data
+val get_state_type_global   = snd o get_data_global
+fun upd_state_type f        = map_data (fn (tab,t) => (tab, f t))
+fun upd_state_type_global f = map_data_global (fn (tab,t) => (tab, f t))
+
+
+fun is_program_variable name thy = Symtab.defined((fst o get_data_global) thy) name
+
+fun is_global_program_variable name thy = case Symtab.lookup((fst o get_data_global) thy) name of
+                                             SOME(global_var _) => true
+                                           | _ => false
+
+fun is_local_program_variable name thy = case Symtab.lookup((fst o get_data_global) thy) name of
+                                             SOME(local_var _) => true
+                                           | _ => false
+
+fun declare_state_variable_global f field thy  =  
+             let val Const(name,Type("fun",ty::_)) = Syntax.read_term_global thy field
+             in  (map_data_global (apfst (Symtab.update_new(name,f ty))) (thy)
+                 handle Symtab.DUP _ => error("multiple declaration of global var"))
+             end;
+
+fun declare_state_variable_local f field ctxt  = 
+             let val Const(name,Type("fun",ty::_)) = Syntax.read_term_global 
+                                                        (Context.theory_of ctxt) field
+             in  (map_data (apfst (Symtab.update_new(name,f ty)))(ctxt)
+                 handle Symtab.DUP _ => error("multiple declaration of global var"))
+             end;
+(*
+
+fun declare_state_variable_local field ctxt  = (map_data (apfst(fn {tab=t,maxano=x} => 
+
+val Const(name,Type("fun",a::R)) = Syntax.read_term @{context} "tm"
+*)
+end
+
+*}
+
+ML{* 
+local open StateMgt_core in
+
+val S = List.foldr (fn ((f,_,_), thy) 
+                    => declare_state_variable_global global_var (Binding.name_of f) thy)  
+
+end
+*}
+
+ML\<open>\<close>
+
+ML{*
+val SPY = Unsynchronized.ref([]:(binding * typ * mixfix)list)
+
+fun read_parent NONE ctxt = (NONE, ctxt)
+  | read_parent (SOME raw_T) ctxt =
+      (case Proof_Context.read_typ_abbrev ctxt raw_T of
+        Type (name, Ts) => (SOME (Ts, name), fold Variable.declare_typ Ts ctxt)
+      | T => error ("Bad parent record specification: " ^ Syntax.string_of_typ ctxt T));
+
+fun read_fields raw_fields ctxt =
+  let
+    val Ts = Syntax.read_typs ctxt (map (fn (_, raw_T, _) => raw_T) raw_fields);
+    val fields = map2 (fn (x, _, mx) => fn T => (x, T, mx)) raw_fields Ts;
+    val ctxt' = fold Variable.declare_typ Ts ctxt;
+  in (fields, ctxt') end;
+
+fun add_record_cmd overloaded is_global_kind (raw_params, binding) raw_parent raw_fields thy =
+  let
+    val ctxt = Proof_Context.init_global thy;
+    val params = map (apsnd (Typedecl.read_constraint ctxt)) raw_params;
+    val ctxt1 = fold (Variable.declare_typ o TFree) params ctxt;
+    val (parent, ctxt2) = read_parent raw_parent ctxt1;
+    val (fields, ctxt3) = read_fields raw_fields ctxt2;
+    val params' = map (Proof_Context.check_tfree ctxt3) params;
+    val declare = StateMgt_core.declare_state_variable_global
+    fun insert_var ((f,_,_), thy') = 
+            if is_global_kind then declare StateMgt_core.global_var (Binding.name_of f) thy'
+            else declare StateMgt_core.local_var (Binding.name_of f) thy'
+    val _ = (SPY := fields)
+  in thy |> Record.add_record overloaded (params', binding) parent fields 
+         |> (fn thy =>  List.foldr insert_var (thy) (fields))
+  end;
+
+fun typ_2_string_raw (Type(s,S)) = 
+        let  val h = if null S then "" else enclose "(" ")" (commas (map typ_2_string_raw ( S))) ;
+        in h ^ s end
+   |typ_2_string_raw (TFree(s,_))  = s 
+   |typ_2_string_raw (TVar((s,n),_))  = s^(Int.toString n) ;
+
+fun typ_2_string_raw (Type(s,S)) = 
+        let val front = fst o split_last
+            val h = if null S then "" else enclose "(" ")" (commas (map typ_2_string_raw (front S))) ;
+        in h ^ (Long_Name.qualifier s) end
+   |typ_2_string_raw (TFree(s,_))  = s 
+   |typ_2_string_raw (TVar((s,n),_))  = s^(Int.toString n) ;
+
+
+
+fun new_state_record  is_global_kind (raw_params, binding)  raw_fields thy =
+    let val _ = writeln (typ_2_string_raw (StateMgt_core.get_state_type_global thy))
+        val raw_parent = SOME(typ_2_string_raw (StateMgt_core.get_state_type_global thy))
+    in  add_record_cmd {overloaded = false} is_global_kind (raw_params, binding) raw_parent raw_fields thy
+    end
+
+val _ =
+  Outer_Syntax.command @{command_keyword global_vars} "define global state record"
+    ((Parse.type_args_constrained -- Parse.binding) -- Scan.repeat1 Parse.const_binding
+    >> (fn (x, z) => Toplevel.theory (new_state_record true x  z)));
+
+val _ =
+  Outer_Syntax.command @{command_keyword local_vars} "define local state record"
+    ((Parse.type_args_constrained -- Parse.binding) -- Scan.repeat1 Parse.const_binding
+    >> (fn (x, z) => Toplevel.theory (new_state_record false x  z)));
+
+
+*}
+
+ML\<open>@{command_keyword "global_vars"}\<close>
+
+section\<open>Monadic Presentation of Assignments (based on Records) \<close>
+
+
+text\<open> ... and we provide syntactic sugar via cartouches \<close>
+
+text\<open> Basic Symbolic execution rules. As they are equalities, they can also
+be used as program optimization rules. \<close>
+
+lemma exec_assign  : 
+assumes "\<not> exec_stop \<sigma>"
+shows "(\<sigma> \<Turnstile> ( _ \<leftarrow> assign f; M)) = ((f \<sigma>) \<Turnstile>  M)"
+by (simp add: assign_def assms exec_bind_SE_success)
+    
+lemma exec_assign'  : 
+assumes "exec_stop \<sigma>"
+shows "(\<sigma> \<Turnstile> ( _ \<leftarrow> assign f; M)) = (\<sigma> \<Turnstile>  M)"
+by (simp add: assign_def assms exec_bind_SE_success)     
+
+lemmas exec_assignD = exec_assign[THEN iffD1]
+
+lemmas exec_assignD' = exec_assign'[THEN iffD1]
+
+lemma exec_If\<^sub>C_If\<^sub>S\<^sub>E  : 
+assumes "\<not> exec_stop \<sigma>"
+shows  " ((if\<^sub>C P then B\<^sub>1 else B\<^sub>2 fi))\<sigma> = ((if\<^sub>S\<^sub>E P then B\<^sub>1 else B\<^sub>2 fi)) \<sigma> "
+  unfolding if_SE_def MonadSE.if_SE_def Symbex_MonadSE.valid_SE_def MonadSE.bind_SE'_def
+  by (simp add: assms bind_SE_def if_C_def)
+    
+    
+lemma valid_exec_If\<^sub>C  : 
+assumes "\<not> exec_stop \<sigma>"
+shows  "(\<sigma> \<Turnstile> (if\<^sub>C P then B\<^sub>1 else B\<^sub>2 fi);-M) = (\<sigma> \<Turnstile> (if\<^sub>S\<^sub>E P then B\<^sub>1 else B\<^sub>2 fi);-M)"
+  by (meson assms exec_If\<^sub>C_If\<^sub>S\<^sub>E valid_bind'_cong)
+
+
+      
+lemma exec_If\<^sub>C'  : 
+assumes "exec_stop \<sigma>"
+shows  "(\<sigma> \<Turnstile> (if\<^sub>C P then B\<^sub>1 else B\<^sub>2 fi);-M) = (\<sigma> \<Turnstile> M)"    
+  unfolding if_SE_def MonadSE.if_SE_def Symbex_MonadSE.valid_SE_def MonadSE.bind_SE'_def bind_SE_def
+    by (simp add: assms if_C_def)
+    
+lemma exec_While\<^sub>C'  : 
+assumes "exec_stop \<sigma>"
+shows  "(\<sigma> \<Turnstile> (while\<^sub>C P do B\<^sub>1 od);-M) = (\<sigma> \<Turnstile> M)"    
+  unfolding while_C_def MonadSE.if_SE_def Symbex_MonadSE.valid_SE_def MonadSE.bind_SE'_def bind_SE_def
+  apply simp using assms by blast    
+    
+text\<open> Syntactic sugar via cartouches \<close>
+
+ML \<open>
+val SPY = Unsynchronized.ref(Bound 0)
+  local
+    fun app_sigma db tm ctxt = case tm of
+        Const(name, _) => if StateMgt_core.is_program_variable name (Proof_Context.theory_of ctxt) 
+                          then tm $ (Bound db) (* lifting *)
+                          else tm              (* no lifting *)
+      | Free _ => tm
+      | Var _ => tm
+      | Bound _ => tm
+      | Abs (x, a, tm') => Abs(x, a, app_sigma (db+1) tm' ctxt)
+      | t1 $ t2 => (app_sigma db t1 ctxt) $ (app_sigma db t2 ctxt)
+      
+    fun mk_assign t1 ctxt = case t1 of
+        (Const("_type_constraint_",_)) $ (Const (name,ty))    => 
+                          if StateMgt_core.is_program_variable name (Proof_Context.theory_of ctxt) 
+                          then Const(name^Record.updateN, ty)
+                          else raise TERM ("mk_assign", [t1])
+      | _ => raise TERM ("mk_assign", [t1])
+
+    fun transform_term tm ctxt =
+            case tm of
+               Const("Clean.syntax_assign",_) $ t1 $ t2 =>
+                  Const(@{const_name "assign"},dummyT)
+                  $ (Abs ("\<sigma>", dummyT, ((mk_assign t1 ctxt) 
+                                      $ (absdummy dummyT (app_sigma 1 t2 ctxt)) 
+                                      $ (Bound 0))))
+             | _ => Abs ("\<sigma>", dummyT, app_sigma 0 tm ctxt)
+  in
+    fun string_tr ctxt (content:(string * Position.T) -> (string * Position.T) list) (args:term list) : term =
+      let fun err () = raise TERM ("string_tr", args) 
+      in
+        (case args of
+          [(Const (@{syntax_const "_constrain"}, _)) $ (Free (s, _)) $ p] =>
+            (case Term_Position.decode_position p of
+              SOME (pos, _) =>
+              let val txt = Symbol_Pos.implode(content (s,pos))
+                  val tm = Syntax.parse_term ctxt txt
+                  val _ = (SPY := tm)
+                  val tr = transform_term tm ctxt
+                  val ct = Syntax.check_term ctxt tr
+              in
+                ct
+              end
+            | NONE => err ())
+        | _ => err ())
+      end
+  end
+\<close>
+
+syntax "_cartouche_string" :: "cartouche_position \<Rightarrow> string"  ("_")
+
+parse_translation \<open>
+  [(@{syntax_const "_cartouche_string"},
+    (fn ctxt => (string_tr ctxt ((Symbol_Pos.cartouche_content : Symbol_Pos.T list -> Symbol_Pos.T list)
+                 o (Symbol_Pos.explode : string * Position.T -> Symbol_Pos.T list)))) )]
+\<close>
+
+
+section\<open> Tactic Support: we use Eisbach to automate the process. \<close>
+
+txt\<open> Necessary prerequisite: turning ematch and dmatch into a proper Isar Method. \<close>
+(* TODO : this code shoud go to TestGen Method setups *)
+ML\<open>
+val _ =
+  Theory.setup
+   (Method.setup @{binding ematch}
+      (Attrib.thms >> (fn rules => fn ctxt => METHOD (HEADGOAL o (K(ematch_tac ctxt rules)) ))) 
+      "fast elimination matching" #>
+    Method.setup @{binding dmatch}
+      (Attrib.thms >> (fn rules => fn ctxt => METHOD (HEADGOAL o (K(dmatch_tac ctxt rules)) ))) 
+       "fast destruction matching" #>
+    Method.setup @{binding match}
+      (Attrib.thms >> (fn rules => fn ctxt => METHOD (HEADGOAL o (K(match_tac ctxt rules)) )))
+       "resolution based on fast matching")
+\<close>
+
+txt\<open> Various tactics for various coverage criteria \<close>
+
+definition while_k :: "nat \<Rightarrow> (('\<alpha>, '\<sigma>) control_state_ext \<Rightarrow> bool) 
+                        \<Rightarrow> (unit, ('\<alpha>, '\<sigma>) control_state_ext)MON\<^sub>S\<^sub>E 
+                        \<Rightarrow> (unit, ('\<alpha>, '\<sigma>) control_state_ext)MON\<^sub>S\<^sub>E"
+where     "while_k _ \<equiv> while_C"
+
+lemma while_k_SE : "while_C = while_k k"
+by (simp only: while_k_def)
+    
+    
+lemma if\<^sub>C_cond_cong : "f \<sigma> = g \<sigma> \<Longrightarrow> 
+                           (if\<^sub>C f then c else d fi) \<sigma> = 
+                           (if\<^sub>C g then c else d fi) \<sigma>"
+  unfolding if_C_def
+   by simp 
+   
+     
+
+lemma while\<^sub>C_skip [simp]: "(while\<^sub>C (\<lambda> x. False) do c od) = skip\<^sub>S\<^sub>E"
+  apply(rule ext)
+  unfolding while_C_def skip\<^sub>S\<^sub>E_def unit_SE_def
+  apply auto
+  unfolding exec_stop_def skip\<^sub>S\<^sub>E_def unset_break_def bind_SE'_def unit_SE_def bind_SE_def
+  by simp
+  
+
+lemma break_assign_skip [simp]: "break ;- assign f = break"
+  apply(rule ext)
+  unfolding break_def assign_def exec_stop_def bind_SE'_def   bind_SE_def
+  by auto
+
+lemma break_if_skip [simp]: "break ;- (if\<^sub>C b then c else d fi) = break"
+  apply(rule ext)
+  unfolding break_def assign_def exec_stop_def if_C_def bind_SE'_def   bind_SE_def
+  by auto
+    
+                       
+lemma break_while_skip [simp]: "break ;- (while\<^sub>C b do c od) = break"
+  apply(rule ext)
+  unfolding while_C_def skip\<^sub>S\<^sub>E_def unit_SE_def bind_SE'_def bind_SE_def break_def exec_stop_def
+  by simp
+
+    
+lemma unset_break_idem [simp] : "( unset_break ;- unset_break ;- M) = (unset_break ;- M)"
+  apply(rule ext)  unfolding unset_break_def bind_SE'_def bind_SE_def by auto
+    
+    
+method bound_while for n::nat = (simp only: while_k_SE [of n])
+
+
+(* this still holds ... *)
+lemma exec_while\<^sub>C : 
+"(\<sigma> \<Turnstile> ((while\<^sub>C b do c od) ;- M)) = 
+ (\<sigma> \<Turnstile> ((if\<^sub>C b then c ;- (while\<^sub>C b do c od) ;- unset_break else skip\<^sub>S\<^sub>E fi)  ;- M))"
+proof (cases "exec_stop \<sigma>")
+  case True
+  then show ?thesis 
+    by (simp add: True exec_If\<^sub>C' exec_While\<^sub>C')
+next
+  case False
+  then show ?thesis
+    proof (cases "\<not> b \<sigma>")
+      case True
+      then show ?thesis
+        apply(subst valid_bind'_cong)
+        using `\<not> exec_stop \<sigma>` apply simp_all
+        apply (auto simp: skip\<^sub>S\<^sub>E_def unit_SE_def)
+          apply(subst while_C_def, simp)
+         apply(subst bind'_cong)
+         apply(subst MonadSE.while_SE_unfold)
+          apply(subst if\<^sub>S\<^sub>E_cond_cong [of _ _ "\<lambda>_. False"])
+          apply simp_all
+        apply(subst if\<^sub>C_cond_cong [of _ _ "\<lambda>_. False"], simp add: )
+        apply(subst exec_If\<^sub>C_If\<^sub>S\<^sub>E,simp_all)
+        by (simp add: exec_stop_def unset_break_def)
+    next
+      case False
+      have * : "b \<sigma>"  using False by auto
+      then show ?thesis
+           unfolding while_k_def 
+           apply(subst  while_C_def)
+           apply(subst  if_C_def)
+           apply(subst  valid_bind'_cong)
+            apply (simp add: `\<not> exec_stop \<sigma>`)
+           apply(subst  (2) valid_bind'_cong)
+            apply (simp add: `\<not> exec_stop \<sigma>`)
+            apply(subst MonadSE.while_SE_unfold)
+            apply(subst valid_bind'_cong)
+            apply(subst bind'_cong)
+             apply(subst if\<^sub>S\<^sub>E_cond_cong [of _ _ "\<lambda>_. True"])
+              apply(simp_all add:   `\<not> exec_stop \<sigma>` )
+            apply(subst bind_assoc', subst bind_assoc')
+            proof(cases "c \<sigma>")
+              case None
+              then show "(\<sigma> \<Turnstile> c;-((while\<^sub>S\<^sub>E (\<lambda>\<sigma>. \<not> exec_stop \<sigma> \<and> b \<sigma>) do c od);-unset_break);-M) =
+                         (\<sigma> \<Turnstile> c;-(while\<^sub>C b do c od) ;- unset_break ;- M)"
+                by (simp add: bind_SE'_def exec_bind_SE_failure)
+            next
+              case (Some a)
+              then show "(\<sigma> \<Turnstile> c ;- ((while\<^sub>S\<^sub>E (\<lambda>\<sigma>. \<not> exec_stop \<sigma> \<and> b \<sigma>) do c od);-unset_break);-M) =
+                         (\<sigma> \<Turnstile> c ;- (while\<^sub>C b do c od) ;- unset_break ;- M)"
+                apply(insert `c \<sigma> = Some a`, subst (asm) surjective_pairing[of a])
+                apply(subst exec_bind_SE_success2, assumption)
+                apply(subst exec_bind_SE_success2, assumption)
+                proof(cases "exec_stop (snd a)")
+                  case True
+                  then show "(snd a \<Turnstile>((while\<^sub>S\<^sub>E (\<lambda>\<sigma>. \<not> exec_stop \<sigma> \<and> b \<sigma>) do c od);-unset_break);-M)=
+                             (snd a \<Turnstile> (while\<^sub>C b do c od) ;- unset_break ;- M)"
+                       by (metis (no_types, lifting) bind_assoc' exec_While\<^sub>C' exec_skip if_SE_D2' 
+                                                  skip\<^sub>S\<^sub>E_def while_SE_unfold)
+                next
+                  case False
+                  then show "(snd a \<Turnstile> ((while\<^sub>S\<^sub>E(\<lambda>\<sigma>. \<not>exec_stop \<sigma> \<and> b \<sigma>) do c od);-unset_break);-M)=
+                             (snd a \<Turnstile> (while\<^sub>C b do c od) ;- unset_break ;- M)"
+                          unfolding  while_C_def
+                          by(subst (2) valid_bind'_cong,simp)(simp)
+                qed       
+            qed  
+    qed
+qed
+(* ... although it is, oh my god, amazingly complex to prove. *)
+  
+corollary exec_while_k : 
+"(\<sigma> \<Turnstile> ((while_k (Suc n) b c) ;- M)) = 
+ (\<sigma> \<Turnstile> ((if\<^sub>C b then c ;- (while_k n b c) ;- unset_break else skip\<^sub>S\<^sub>E fi)  ;- M))"
+  by (metis exec_while\<^sub>C while_k_def)
+    
+
+lemmas exec_while_kD = exec_while_k[THEN iffD1]
+
+named_theorems memory_theory
+method memory_theory = (simp only: memory_theory MonadSE.bind_assoc')
+method norm = (auto dest!: assert_D)
+
+(* Remark: if instead of a recursive call, we use "+", this corresponds to recursing only on the
+   first goal, and thus does not work with nested loops *)
+method loop_coverage_steps methods simp_mid =
+  ((ematch assume_E')
+    | (ematch if_SE_execE'', simp_mid?)
+    | (dmatch exec_while_kD)
+    | (dmatch exec_skipD)
+    | (dmatch exec_assignD')
+  ); (loop_coverage_steps simp_mid)?
+method loop_coverage for n::nat methods simp_mid simp_end =
+       (bound_while n)?, loop_coverage_steps simp_mid, simp_end?
+  
+method branch_and_loop_coverage for n::nat uses mt = loop_coverage n memory_theory simp_all
+method mcdc_and_loop_coverage for n::nat = loop_coverage n auto auto
+
+
+(* method mcdc_and_loop_coverage for n::nat = loop_coverage n norm norm *)
+
+method loop_coverage_positive_branch_steps =
+  ((ematch assume_E')
+    | (ematch if_SE_execE''_pos, memory_theory?)
+    | (dmatch exec_while_kD, ematch if_SE_execE'', memory_theory?)
+    | (dmatch exec_skipD)
+    | (dmatch exec_assignD')
+  ); loop_coverage_positive_branch_steps?
+method loop_coverage_positive_branch for n::nat =
+  (bound_while n)?, loop_coverage_positive_branch_steps, simp_all?
+
+end
+
+  
+  
